src/proofs/no_slashable_attestations/supporting_lemmas/ind_inv_implies_safety/core_proofs.dfy
@@ -53,8 +53,8 @@ module Core_Proofs
     requires a.data.slot < a'.data.slot
     requires inv_sent_validity_predicate_only_for_slots_stored_in_att_slashing_db_hist(dv)
     requires inv_all_validity_predicates_are_stored_in_att_slashing_db_hist(dv)
-    requires pred_4_1_g_i(dv)
-    requires pred_4_1_g_iii(dv)
+    requires inv_sent_validity_predicate_is_based_on_rcvd_duty_and_slashing_db_in_hist(dv)
+    requires inv_sent_validity_predicate_is_based_on_rcvd_duty_and_slashing_db_in_histii(dv)
     requires inv_queued_att_duty_is_rcvd_duty0(dv)
     // requires inv_queued_att_duty_is_rcvd_duty1(dv)
     ensures && !is_slashable_attestation_data_eth_spec(a.data, a'.data)
@@ -174,8 +174,8 @@ module Core_Proofs
     requires concl_exists_honest_dvc_that_sent_att_share_for_submitted_att(dv)
     requires pred_data_of_att_share_is_decided_value(dv)
     requires inv_decided_value_of_consensus_instance_is_decided_by_quorum(dv)    
-    requires pred_4_1_g_i(dv)
-    requires pred_4_1_g_iii(dv)
+    requires inv_sent_validity_predicate_is_based_on_rcvd_duty_and_slashing_db_in_hist(dv)
+    requires inv_sent_validity_predicate_is_based_on_rcvd_duty_and_slashing_db_in_histii(dv)
     requires && a in dv.all_attestations_created
              && is_valid_attestation(a, dv.dv_pubkey)
     requires && a' in dv.all_attestations_created
@@ -212,8 +212,8 @@ module Core_Proofs
     requires concl_exists_honest_dvc_that_sent_att_share_for_submitted_att(dv)
     requires pred_data_of_att_share_is_decided_value(dv)
     requires inv_decided_value_of_consensus_instance_is_decided_by_quorum(dv)    
-    requires pred_4_1_g_i(dv)
-    requires pred_4_1_g_iii(dv)
+    requires inv_sent_validity_predicate_is_based_on_rcvd_duty_and_slashing_db_in_hist(dv)
+    requires inv_sent_validity_predicate_is_based_on_rcvd_duty_and_slashing_db_in_histii(dv)
     requires && a in dv.all_attestations_created
              && is_valid_attestation(a, dv.dv_pubkey)
     requires && a' in dv.all_attestations_created
@@ -256,8 +256,8 @@ module Core_Proofs
     requires concl_exists_honest_dvc_that_sent_att_share_for_submitted_att(dv)
     requires pred_data_of_att_share_is_decided_value(dv)
     requires inv_decided_value_of_consensus_instance_is_decided_by_quorum(dv)    
-    requires pred_4_1_g_i(dv)
-    requires pred_4_1_g_iii(dv)
+    requires inv_sent_validity_predicate_is_based_on_rcvd_duty_and_slashing_db_in_hist(dv)
+    requires inv_sent_validity_predicate_is_based_on_rcvd_duty_and_slashing_db_in_histii(dv)
     requires && a in dv.all_attestations_created
              && is_valid_attestation(a, dv.dv_pubkey)
     requires && a' in dv.all_attestations_created
